src/StateCalculusTacticTest.v
@@ -14,8 +14,7 @@ Section Tests.
   Context {vars: Type}.
   Context {varset: set vars var}.
 
-  Ltac state_calc_instantiation := state_calc var val.
-  Ltac state_calc := state_calc_instantiation.
+  Ltac state_calc := state_calc_generic var val.
 
   Lemma extends_refl: forall s, extends s s.
   Proof. state_calc. Qed.
